End to end fib demo without proving correctness

compiler/src/examples/FibCompiled.v
@@ -98,28 +98,266 @@ Section FibCompiled.
       end
     end.
 
-  Definition regb : Register := 2.
-
   Existing Instance Demos.Fibonacci.ZNames.Inst.
-                                  
-  Axiom fib_program_logic: forall n t m l mc,
-     n < BinInt.Z.pow_pos 2 32 ->
-     Semantics.exec map.empty (fib_ExprImp n) t m l mc (
-                      fun t' m ' l' mc' =>
-                        bedrock2.MetricLogging.instructions mc' <= bedrock2.MetricLogging.instructions mc + 34 * n + 39 /\
-                        exists (result: Utility.word),
-                          word.unsigned result = (fib (Z.to_nat n)) /\
-                          map.get l' regb = Some result).
 
-  Lemma fib_demo: forall n,
+  Local Notation instructionsH := (bedrock2.MetricLogging.instructions).
+  
+  Fixpoint get_next_bb exprimp :=
+    match exprimp with
+    | cmd.seq _ x => get_next_bb x
+    | _ => exprimp
+    end.
+
+  Definition get_while_body exprimp :=
+    match exprimp with
+    | cmd.while _ x => x
+    | _ => exprimp
+    end.
+
+  Definition fib_while n := get_next_bb (fib_ExprImp n).
+
+  Definition fib_while_body n := get_while_body (fib_while n).
+
+  Ltac destruct_hyp :=
+    repeat match goal with
+           | H : _ /\ _ |- _ => destruct H
+           end.
+
+  Ltac eval_fib_var_names :=
+    cbv [Demos.Fibonacci.a
+           Demos.Fibonacci.b
+           Demos.Fibonacci.c
+           Demos.Fibonacci.i
+           Demos.Fibonacci.ZNames.Inst] in *.
+
+  Lemma fib_bounding_metrics_body: forall t m (l : locals) mc a b i n,
+      map.get l Demos.Fibonacci.a = Some a ->
+      map.get l Demos.Fibonacci.b = Some b ->
+      map.get l Demos.Fibonacci.i = Some i ->
+      exec map.empty (fib_while_body n) t m l mc (fun t' m' l' mc' =>
+                                                    map.get l' Demos.Fibonacci.a = Some b /\
+                                                    map.get l' Demos.Fibonacci.b = Some (word.add a b) /\
+                                                    map.get l' Demos.Fibonacci.i = Some (word.add i (word.of_Z 1)) /\
+                                                    instructionsH mc' - instructionsH mc = 21).
+  Proof.
+    intros.
+    cbv [fib_ExprImp get_next_bb get_while_body fib_while fib_while_body].
+    eapply @exec.seq with (mid := (fun t' m' l' mc' =>
+                                     t' = t /\
+                                     map.get l' Demos.Fibonacci.a = Some a /\
+                                     map.get l' Demos.Fibonacci.b = Some b /\
+                                     map.get l' Demos.Fibonacci.c = Some (word.add a b) /\
+                                     map.get l' Demos.Fibonacci.i = Some i /\
+                                     instructionsH mc' = instructionsH mc + 5)).
+    - eapply @exec.set.
+      + unfold eval_expr. eval_fib_var_names.
+        rewrite H. rewrite H0. eauto.
+      + repeat split.
+        * rewrite map.get_put_diff; [assumption | discriminate].
+        * rewrite map.get_put_diff; [assumption | discriminate].
+        * apply map.get_put_same.
+        * rewrite map.get_put_diff; [assumption | discriminate].
+        * simpl. Lia.lia.
+    - intros.
+      eapply @exec.seq with (mid := (fun t' m' l' mc' =>
+                                       t' = t /\
+                                       map.get l' Demos.Fibonacci.a = Some b /\
+                                       map.get l' Demos.Fibonacci.b = Some b /\
+                                       map.get l' Demos.Fibonacci.c = Some (word.add a b) /\
+                                       map.get l' Demos.Fibonacci.i = Some i /\
+                                       instructionsH mc' = instructionsH mc + 7)).
+      + destruct_hyp.
+        eapply @exec.set.
+        * unfold eval_expr. eval_fib_var_names.
+          rewrite H4. eauto.
+        * repeat split.
+          -- assumption.
+          -- apply map.get_put_same.
+          -- rewrite map.get_put_diff; [assumption | discriminate].
+          -- rewrite map.get_put_diff; [assumption | discriminate].
+          -- rewrite map.get_put_diff; [assumption | discriminate].
+          -- simpl. Lia.lia.
+      + intros.
+        eapply @exec.seq with (mid := (fun t' m' l' mc' =>
+                                         t' = t /\
+                                         map.get l' Demos.Fibonacci.a = Some b /\
+                                         map.get l' Demos.Fibonacci.b = Some (word.add a b) /\
+                                         map.get l' Demos.Fibonacci.c = Some (word.add a b) /\
+                                         map.get l' Demos.Fibonacci.i = Some i /\
+                                         instructionsH mc' = instructionsH mc + 9)).
+        * destruct_hyp.
+          eapply @exec.set.
+          -- unfold eval_expr. eval_fib_var_names.
+             rewrite H6. eauto.
+          -- repeat split.
+             ++ assumption.
+             ++ rewrite map.get_put_diff; [assumption | discriminate].
+             ++ apply map.get_put_same.
+             ++ rewrite map.get_put_diff; [assumption | discriminate].
+             ++ rewrite map.get_put_diff; [assumption | discriminate].
+             ++ simpl. Lia.lia.
+        * intros.
+          destruct_hyp.
+          eapply @exec.set.
+          -- unfold eval_expr. eval_fib_var_names.
+             rewrite H8. eauto.
+          -- repeat split.
+             ++ rewrite map.get_put_diff; [assumption | discriminate].
+             ++ rewrite map.get_put_diff; [assumption | discriminate].
+             ++ apply map.get_put_same.
+             ++ simpl. Lia.lia.
+  Qed.
+
+  Lemma fib_bounding_metrics_while: forall (n : nat) (iter : nat) t m (l : locals) mc a b,
+      (Z.of_nat n) < 2 ^ 32 ->
+      (iter <= n)%nat ->
+      map.get l Demos.Fibonacci.a = Some a ->
+      map.get l Demos.Fibonacci.b = Some b ->
+      map.get l Demos.Fibonacci.i = Some (word.of_Z ((Z.of_nat n) - (Z.of_nat iter)) : word) ->
+      exec map.empty (fib_while (Z.of_nat n)) t m l mc (fun t' m' l' mc' =>
+                                                          instructionsH mc' <= instructionsH mc + (Z.of_nat iter) * 34 + 12).
+  Proof.
+    induction iter.
+    - intros.
+      eapply @exec.while_false.
+      + unfold eval_expr. eval_fib_var_names.
+        rewrite H3. eauto.
+      + simpl. destruct_one_match.
+        * rewrite Z.sub_0_r in E. pose proof Z.ltb_irrefl.
+          specialize (H4 (Z.of_nat n mod 2 ^ 32)). rewrite H4 in E. discriminate.
+        * auto.
+      + simpl. Lia.lia.
+    - intros.
+      eapply @exec.while_true.
+      + unfold eval_expr. eval_fib_var_names.
+        rewrite H3. eauto.
+      + simpl. destruct_one_match.
+        * simpl. rewrite Zdiv.Zmod_1_l.
+          { discriminate. }
+          { cbv. reflexivity. }
+        * rewrite Z.mod_small in E; [| blia ].
+          rewrite Z.mod_small in E; [| blia ].
+          assert (Z.of_nat n - Z.of_nat (S iter) < Z.of_nat n) by Lia.lia.
+          apply Z.ltb_lt in H4.
+          rewrite H4 in E. discriminate.
+      + eapply fib_bounding_metrics_body with (n := Z.of_nat n); eauto.
+      + intros. destruct H4. destruct H5. destruct H6.
+        eval_fib_var_names.
+        assert (iter <= n)%nat by Lia.lia.
+        assert (map.get l' 4 = Some (word.of_Z (Z.of_nat n - Z.of_nat iter))). {
+          rewrite H6. f_equal.
+          apply word.unsigned_inj.
+          rewrite word.unsigned_add. rewrite !word.unsigned_of_Z.
+          f_equal. unfold word.wrap. change (1 mod 2 ^ Semantics.width) with 1. simpl.
+          rewrite Z.mod_small; blia.
+        }
+        specialize IHiter with (1 := H) (2 := H8) (3 := H4) (4 := H5) (5 := H9).
+        simpl in H7.
+        unfold_MetricLog. simpl in IHiter.
+        eapply weaken_exec in IHiter.
+        * eapply IHiter.
+        * intros. simpl in *. Lia.lia.
+  Qed.
+
+  Lemma fib_bounding_metrics: forall (n: nat) t m (l : locals) mc,
+      (Z.of_nat n) < BinInt.Z.pow_pos 2 32 ->
+      exec map.empty (fib_ExprImp (Z.of_nat n)) t m l mc (fun t' m ' l' mc' =>
+        instructionsH mc' <= instructionsH mc + (Z.of_nat n) * 34 + 39).
+  Proof.
+    intros.
+    unfold fib_ExprImp.
+    eapply @exec.seq with (mid := (fun t' m' l' mc' =>
+                                     t' = t /\
+                                     map.get l' Demos.Fibonacci.a = Some (word.of_Z 0) /\
+                                     instructionsH mc' = instructionsH mc + 9)).
+    - eapply @exec.set.
+      + unfold eval_expr. eauto.
+      + repeat split.
+        * apply map.get_put_same.
+        * simpl. Lia.lia.
+    - intros.
+      destruct H0. destruct H1.
+      eapply @exec.seq with (mid := (fun t' m' l' mc' =>
+                                       t' = t /\
+                                       map.get l' Demos.Fibonacci.a = Some (word.of_Z 0) /\
+                                       map.get l' Demos.Fibonacci.b = Some (word.of_Z 1) /\
+                                       instructionsH mc' = instructionsH mc + 18)).
+      + eapply @exec.set.
+        * unfold eval_expr. eauto.
+        * repeat split.
+          -- assumption.
+          -- rewrite map.get_put_diff; [assumption | discriminate].
+          -- apply map.get_put_same.
+          -- simpl. Lia.lia.
+      + intros.
+        destruct H3. destruct H4. destruct H5.
+        eapply @exec.seq with (mid := (fun t' m' l' mc' =>
+                                         t' = t /\
+                                         map.get l' Demos.Fibonacci.a = Some (word.of_Z 0) /\
+                                         map.get l' Demos.Fibonacci.b = Some (word.of_Z 1) /\
+                                         map.get l' Demos.Fibonacci.i = Some (word.of_Z 0) /\
+                                         instructionsH mc' = instructionsH mc + 27)).
+        * eapply @exec.set.
+          -- unfold eval_expr. eauto.
+          -- repeat split.
+             ++ assumption.
+             ++ rewrite map.get_put_diff; [assumption | discriminate].
+             ++ rewrite map.get_put_diff; [assumption | discriminate].
+             ++ apply map.get_put_same.
+             ++ simpl. Lia.lia.
+        * intros.
+          destruct H7. destruct H8. destruct H9. destruct H10.
+          assert (n <= n)%nat by auto.
+          pose proof fib_bounding_metrics_while as HWhile.
+          specialize HWhile with (iter := n) (n := n).
+          replace (Z.of_nat n - Z.of_nat n) with 0 in HWhile by Lia.lia.
+          specialize HWhile with (1 := H) (2 := H12) (3 := H8) (4 := H9) (5 := H10).
+          specialize (HWhile t'1 m'1 mc'1).
+          eapply weaken_exec in HWhile.
+          -- apply HWhile.
+          -- intros. simpl. Lia.lia.
+  Qed.
+                                  
+  Axiom fib_program_correct: forall n t m l mc,
+      0<= n < BinInt.Z.pow_pos 2 32 ->
+      Semantics.exec map.empty (fib_ExprImp n) t m l mc (
+                       fun t' m ' l' mc' =>
+                         exists (result: Utility.word),
+                           word.unsigned result = (fib (Z.to_nat n)) /\
+                           map.get l' Demos.Fibonacci.b = Some result).
+    
+
+  Lemma fib_program_correct_bounded: forall n t m l mc,
+      0 <= n < BinInt.Z.pow_pos 2 32 ->
+      Semantics.exec map.empty (fib_ExprImp n) t m l mc (
+                       fun t' m ' l' mc' =>
+                         instructionsH mc' <= instructionsH mc + n * 34 + 39 /\
+                         exists (result: Utility.word),
+                           word.unsigned result = (fib (Z.to_nat n)) /\
+                           map.get l' Demos.Fibonacci.b = Some result).
+  Proof.
+    intros.
+    pose proof fib_program_correct.
+    pose proof fib_bounding_metrics.
+    specialize H0 with (1 := H).
+    specialize H1 with (n := Z.to_nat n).
+    rewrite Z2Nat.id in H1; [|blia].
+    destruct H.
+    specialize H1 with (1 := H2).
+    eapply intersect_exec.
+    + eapply H1.
+    + eapply H0.
+  Qed.    
+
+  Lemma fib_compiled: forall n,
     0 <= n <= 60 ->
     runsToNonDet.runsTo (mcomp_sat run1)
                         (programmedMachine n)
                         (fun (finalL: RiscvMachine) =>
                            exists (result: Utility.word),
-                             map.get finalL.(getRegs) regb = Some result /\
+                             map.get finalL.(getRegs) Demos.Fibonacci.b = Some result /\
                              word.unsigned result = (fib (Z.to_nat n)) /\
-                             finalL.(getMetrics).(instructions) <= 34 * n + 39).
+                             finalL.(getMetrics).(instructions) <= n * 34 + 39).
   Proof.
     intros.
     eapply runsToNonDet.runsTo_weaken.
@@ -145,11 +383,7 @@ Section FibCompiled.
         end.
         simpl. blia.
       + cbv [Pipeline.ext_guarantee pipeline_params]. exact I.
-      + eapply ExprImp.weaken_exec; [eapply fib_program_logic|].
-        * match goal with
-          | |- _ < ?x => let r := eval cbv in x in change x with r
-          end.
-          blia.
+      + eapply ExprImp.weaken_exec; [eapply fib_program_correct_bounded; cbn; blia|].
         * intros.
           match goal with
           | H: _ ?t ?m ?l ?mc |- _ ?t ?m ?l ?mc => apply H
@@ -173,7 +407,11 @@ Section FibCompiled.
         repeat match goal with
                | H: _ /\ _ |- _ => destruct H
                end.
-        eapply Z.le_trans; [eassumption|assumption].
+        eapply Z.le_trans.
+        * eassumption.
+        * assumption.
   Qed.
+
+  Print Assumptions fib_compiled.
 
 End FibCompiled.
